Add Arrow ripple carry adder (#152)

cava/arrow-examples/ArrowAdder.v
@@ -21,16 +21,18 @@ Require Import Cava.Arrow.Instances.Combinational.
 Require Import Coq.Strings.String.
 Local Open Scope string_scope.
 
-From Coq Require Import Lists.List.
+From Coq Require Import Lists.List NArith Lia.
 Import ListNotations.
 
 Section definition.
   Import KappaNotation.
 
-  Variable var: Kind -> Kind -> Type.
+  Context {var: Kind -> Kind -> Type}.
 
   Definition halfAdder
   : kappa_sugared var << Bit, Bit, Unit >> <<Bit, Bit>> :=
+    (* The bracket pairing `<[` `]>` opens a circuit expression scope, 
+    see readme.md for more information *) 
   <[ \ a b =>
     let part_sum = xor a b in
     let carry = and a b in
@@ -41,15 +43,124 @@ Section definition.
   : kappa_sugared var << Bit, << Bit, Bit >>, Unit >> <<Bit, Bit>> :=
   <[ \ cin ab =>
     let '(a,b) = ab in
+    (* Since 'halfAdder' is in the larger Coq scope, and is not a local variable,
+    they must be escaped with ! See the readme.md in this file for more explanation*)
     let '(abl, abh) = !halfAdder a b in
     let '(abcl, abch) = !halfAdder abl cin in
     let cout = xor abh abch in
     (abcl, cout)
   ]>.
 
+  (* Combinators *)
+  Definition below {A B C D E F G: Kind}
+    (r: kappa_sugared var << A, B, Unit >> ( G ** D ))
+    (s: kappa_sugared var << G, C, Unit >> ( F ** E ))
+    : kappa_sugared var 
+      << A, (B ** C), Unit >> 
+      << F, (D ** E) >> :=
+  <[ \ a bc =>
+    let '(b, c) = bc in
+    let '(g, d) = !r a b in
+    let '(f, e) = !s g c in
+    (f, (d, e))
+  ]>.
+
+  (* Replicate is a type created by replicating a type n times, 
+  and connecting them by a right imbalanced tuple structure.
+
+  Since the above formulation of 'below' pairs the inputs and outputs 
+  as a tuple (rather requiring the types are equal and appending as a vector), 
+  'replicate' allows us to refer to type arrising from multiple
+  applications of 'below'. 
+  *)
+  Fixpoint replicate A n : Kind :=
+    match n with
+    | O => Unit
+    | S O => A
+    | S n => A ** replicate A n
+    end.
+
+  Program Fixpoint col {A B C: Kind} n
+    (circuit: kappa_sugared var << A, B, Unit >> ( A ** C ))
+    : kappa_sugared var 
+      << A, replicate B (S n), Unit >> 
+      << A, replicate C (S n)>> :=
+    match n with
+    | O => <[ \a b => !circuit a b ]>
+    | S n' =>
+      let column_above := (col n' circuit) in
+      below circuit column_above
+    end.
+
+  Lemma col_cons: forall {A B C}
+    (circuit: kappa_sugared var << A, B, Unit >> ( A ** C )),
+    forall n, col (S n) circuit = below circuit (col n circuit).
+  Proof.
+    intros.
+    auto.
+  Qed.
+
+  Fixpoint interleave n
+    : kappa_sugared var 
+      << Vector (S n) Bit, Vector (S n) Bit, Unit >> 
+      << replicate <<Bit, Bit>> (S n) >> :=
+  match n with
+  (* Since for n = 0 -> Vector 1 Bit, we have to index into the variables to retrieve their values.
+  This is done with familiar 'x[_]' syntax, although numeric constants require prepending with '#'.
+  The index can be any expression. See readme.md for more information.
+  *)
+  | 0 => <[\ x y => (x[#0], y[#0]) ]> 
+  | S n => 
+      <[\ xs ys => 
+      let '(x, xs') = uncons xs in 
+      let '(y, ys') = uncons ys in 
+      ((x, y), (!(interleave n) xs' ys'))
+    ]>
+  end.
+
+  (* As noted above, we use 'replicate' to allow us to refer to a tuple structure of a single type of kind.
+  It would be convenient to interact with this variable as a vector, and so we can write a conversion
+  function : *)
+  Fixpoint productToVec n
+    : kappa_sugared var 
+      << replicate Bit (S n), Unit >> 
+      << Vector (S n) Bit >> :=
+  match n with
+  | 0 => <[\ x => mkVec (x) ]> 
+  | S n => 
+      <[\ xs => 
+      let '(x, xs') = xs in 
+      x :: !(productToVec n) xs'
+    ]>
+  end.
+
+  Definition rippleCarryAdder' (width: nat)
+    : kappa_sugared var
+      << Bit, replicate <<Bit, Bit>> (S width), Unit >> 
+      << Bit, replicate Bit (S width) >> :=
+  <[ !(col width fullAdder) ]>.
+
+  Definition rippleCarryAdder (width: nat)
+    : kappa_sugared var 
+      << Bit, <<Vector (S width) Bit, Vector (S width) Bit>>, Unit >> 
+      << Bit, Vector (S width) Bit >> :=
+  <[ \b xy =>
+    let '(x,y) = xy in
+    let merged = !(interleave _) x y in
+    let '(carry, result) = !(rippleCarryAdder' _) b merged in
+    (carry, !(productToVec _) result)
+    ]>.
+
 End definition.
 
-Definition fullAdder_structure := to_constructive (Desugar fullAdder) (ltac:(auto_kappa_wf)).
+(* The compilation functions performed by this library rely on that the expressions above are well formed.
+Although it is postulated that exotic terms cannot exist in a PHOAS encoding, we provide per instance proofs 
+that later steps consume. *)
+Lemma fullAdder_wf: wf_debrujin [] (Desugar (@fullAdder) _).
+Proof. wf_kappa_via_compute. Qed.
+
+Definition fullAdder_structure := 
+  Eval compute in to_constructive (Desugar (@fullAdder)) (fullAdder_wf).
 
 Lemma fullAdder_is_combinational: wf_combinational (toCava fullAdder_structure _).
 Proof. combinational_obvious. Qed.
@@ -81,7 +192,10 @@ Definition fullAdder_netlist :=
 
 (* Using `evaluate_to_terms` for a nicer extracted value *)
 Definition fullAdder_tb_expected_outputs  : list (bool * bool).
-Proof. evaluate_to_terms fullAdder_structure fullAdder_is_combinational fullAdder_tb_inputs. Defined.
+  (* := (List.map (evaluate (toCava circuit _) wf) inputs) . *)
+Proof. 
+   evaluate_to_terms fullAdder_structure fullAdder_is_combinational fullAdder_tb_inputs. 
+Defined.
 
 Definition fullAdder_tb :=
   testBench "fullAdder_tb" fullAdderInterface
