cava/arrow-examples/readme.md
@@ -1,0 +1,85 @@
+# Intro
+
+Circuit expressions are enclosed in a `<[` `]>` bracket pair.
+
+```
+<[ \x => x ]>
+```
+
+A number of primitive circuits are built-in such as `xor`, and function
+application follows the usual lambda calculus form:
+
+```
+<[ \x y => xor x y ]>
+```
+
+However, our language is actually a restricted form of lambda calculus called
+kappa calulus. The best way to think of this is that you can only express (and typecheck)
+expressions that have a representation as a circuit. So for example, passing functions 
+as arguments is not allowed as it is not representable as a circuit. The benefit being
+that every expression in our language maps directly to a circuit, and component
+instantiation should be observable directly from the syntax.
+
+Other circuit expressions defined in the larger Coq scope are accessible by
+escaping the definition with `!`:
+
+```
+Definition foo := <[\x y => xor x y ]>.
+
+Definition use_foo := <[\x => !foo x x]>.
+```
+
+Each circuit definition (and all expressions with in it) have an input type and
+an output type.
+
+```
+Definition foo : kappa_sugared <<Bit, Bit, Unit>> Bit := <[ xor ]>.
+Definition bar : kappa_sugared <<Bit, Bit, Unit>> Bit := <[\x y => xor x y ]>.
+```
+
+A variable has the `Unit` input type, which is the empty type. So in `bar`
+above, to the right of the binders (`\x y =>`), `x` and `y` both have type `kappa_sugared Unit Bit`.
+
+Bitvector literals are of type `Vector n Bit` and must be prefixed with `#`.
+The width of the literal is given by the type it exists at.
+
+```
+Definition five_zero_bits : kappa_sugared Unit (Vector 5 Bit) := <[ #0 ]>.
+```
+
+# Working with vectors
+
+There are a number of vector functions provided:
+
+- `uncons: Vector (S n) T ~> (T, Vector n T)`
+- `mkVec: T ~> Vector 1 T`
+- `_ :: _: T ~> Vector n T ~> Vector (S n) T`
+
+Additionally indexing can be performed via the familiar `vector [ index ]` syntax, where index can be any circuit expression.
+
+```
+Definition get_zeroth_item : kappa_sugared <<Vector 5 Bit, Unit>> Bit := 
+  <[ \my_vec => my_vec[#0] ]>.
+```
+
+# Higher order functions
+
+What about useful higher-order functions such as `map`? Although we can't pass
+functions as arguments inside a circuit expression, we can write these
+combinators as plain Coq functions acting on circuit expressions:
+
+```
+Fixpoint map {T} n
+  (f : kappa_sugared var <<T, Unit>> T)
+  : kappa_sugared var << Vector (S n) T, Unit >> <<Vector (S n) T>> :=
+match n with
+| 0 => <[ \x => mkVec (!f (x[#0])) ]>
+| S n' =>
+  <[ \xs =>
+      let '(x, xs') = uncons xs in
+      !f x :: (!(map n' f) xs')
+  ]>
+end.
+```
+
+
